Assorted changes to permissions and assertions.

abstract_permissions.v
@@ -7,12 +7,13 @@ free/write/free permissions, fractional permissions, fractional permissions
 with locks) without having to hard-wire these into the memory. *)
 
 (** Permissions form a partial order [(⊆)] with a commutative monoid [(∪)]
-structure. Although the operation [x ∪ y] is only allowed if [x ⊥ y], we
-still treat [(∪)] as a total function to ease formalization. Permissions [x]
-and [y] are ordered [x ⊆ y] in case [y] permits more operations to be performed.
-The operation [(∪)] is used to define the disjoint union of memories. In case
-two memories contain an overlapping cell with permissions [x] and [y]
-respectively, and [x ⊥ y], then the permission of the joined cell is [x ∪ y]. *)
+structure. Although the operation [x ∪ y] only has to be well defined if
+[x ⊥ y], we still treat it as a total function to ease formalization.
+Permissions [x] and [y] are ordered [x ⊆ y] in case [y] permits more operations
+to be performed. The operation [(∪)] is used to define the disjoint union of
+memories. In case two memories contain an overlapping cell with permissions [x]
+and [y] respectively, and [x ⊥ y], then the permission of the joined cell is
+[x ∪ y]. *)
 
 (** It is a good idea to keep fractional permissions in mind. There the order
 [(⊆)] is just the numerical order on the rationals, [(∪)] is ordinary addition,
@@ -33,15 +34,10 @@ write has been performed during a sequence. When a sequence point occurs, the
 permission will be unlocked again using the [perm_unlock] operation. *)
 Inductive pkind := Free | Write | Read | Locked.
 
-Class PermKind P := perm_kind : P → pkind.
-Class PermLock P := perm_lock_ : bool → P → P.
-Notation perm_lock := (perm_lock_ true).
-Notation perm_unlock := (perm_lock_ false).
-
 (** Permission kinds are ordered with respect to the operations that they
 permit. Since read only memory cannot be used for writing (and hence cannot be
-locked), the kinds [Locked] and [Read] are independent with respect to this
-order. *)
+locked), the kinds [Locked] and [Read] are independent from each other with
+respect to this order. *)
 Inductive pkind_subseteq: SubsetEq pkind :=
   | pkind_subseteq_refl k : k ⊆ k
   | Write_subseteq_Free : Write ⊆ Free
@@ -57,15 +53,10 @@ Instance pkind_subseteq_dec (k1 k2 : pkind) : Decision (k1 ⊆ k2).
 Proof.
  refine
   match k1, k2 with
-  | Free, Free => left _
-  | Write, Free => left _
-  | Read, Free => left _
-  | Locked, Free => left _
+  | _, Free => left _
+  | (Locked | Read | Write), Write => left _
   | Locked, Locked => left _
-  | Locked, Write => left _
   | Read, Read => left _
-  | Read, Write => left _
-  | Write, Write => left _
   | _, _ => right _
   end; first [by constructor | by inversion 1].
 Defined.
@@ -107,170 +98,200 @@ Lemma not_Locked_weaken k1 k2 :
 Proof. intros Hk1 ?. contradict Hk1. subst. by apply subseteq_Locked. Qed.
 
 (** * The interface for permissions *)
+Local Unset Elimination Schemes.
+
 (** The interface for permissions is slightly underspecified so as to allow for
 a broad variety of implementations. In particular, we only require the
 [mem_unlock] operation to actually unlock the permission, whereas the [mem_lock]
-operation is not required to really lock the permission. This is to allow the
-unit type, that models a system without permissions, as a satisfying
-implementation. *)
+operation is not required to really lock the permission. This is to allow an
+implementation that does not assign undefined behavior to sequence point
+violations. *)
 
 (** The laws relating [(⊆)], [(⊥)] and [(∪)] all correspond to their respective
-counterpart on the memory that is required to hold for it to be used in a
-separation logic. An important property is that only permissions whose kinds is
-[Read] can be joined together with another permission. This is to ensure that
-given two disjoint memories, only their readable parts may overlap, but their
-writable parts do never overlap. *)
-Definition perm_fragment `{Disjoint P} (p : P) := ∃ p', p ⊥ p'.
+counterpart on the memory that is required to hold in a separation logic. An
+important property is that only permissions whose kinds is [Read] can be joined
+together with another permission. This is to ensure that given two disjoint
+memories, only their readable parts may overlap, but their writable parts do
+never. *)
+Class PermissionsOps (P : Set) := {
+  perm_kind : P → pkind;
+  perm_lock_ : bool → P → P;
+  perm_subseteq :> SubsetEq P;
+  perm_disjoint :> Disjoint P;
+  perm_union :> Union P;
+  perm_difference :> Difference P;
+  perm_disjoint_dec (x y : P) :> Decision (x ⊥ y);
+  perm_eq_dec (x y : P) :> Decision (x = y);
+  perm_subseteq_dec (x y : P) :> Decision (x ⊆ y)
+}.
+Arguments perm_kind _ _ _ : simpl never.
+Arguments perm_lock_ _ _ _ _ : simpl never.
+Arguments perm_subseteq _ _ _ _ : simpl never.
+Arguments perm_disjoint _ _ _ _ : simpl never.
+Arguments perm_union _ _ _ _ : simpl never.
+Arguments perm_difference _ _ _ _ : simpl never.
 
-Class Permissions (P : Set)
-    `{PermKind P}
-    `{PermLock P}
-    `{Union P}
-    `{Disjoint P}
-    `{SubsetEq P}
-    `{Difference P}
-    `{∀ x y : P, Decision (x = y)}
-    `{∀ x y : P, Decision (x ⊥ y)}
-    `{∀ x y : P, Decision (x ⊆ y)} : Prop := {
+Notation perm_lock := (perm_lock_ true).
+Notation perm_unlock := (perm_lock_ false).
+Definition perm_fragment `{PermissionsOps P} (p : P) := ∃ p', p ⊥ p'.
+
+Class Permissions (P : Set) `{PermissionsOps P} : Prop := {
   perm_po :> PartialOrder P;
-  perm_sym :> Symmetric (⊥);
-  perm_kind_preserving x y :
+  perm_sym :> Symmetric (@disjoint P _);
+  perm_kind_preserving (x y : P) :
     x ⊆ y →
     perm_kind x ⊆ perm_kind y;
-  perm_fragment_read x :
+  perm_fragment_read (x : P) :
     perm_fragment x →
     perm_kind x = Read;
-  perm_disjoint_weaken_l x x' y :
+  perm_disjoint_weaken_l (x x' y : P) :
     x ⊥ y → x' ⊆ x → x' ⊥ y;
-  perm_unlock_lock x :
+  perm_unlock_lock (x : P) :
     Write ⊆ perm_kind x →
     perm_unlock (perm_lock x) = x;
-  perm_unlock_other x :
+  perm_unlock_other (x : P) :
     perm_kind x ≠ Locked →
     perm_unlock x = x;
-  perm_unlock_kind x :
+  perm_unlock_kind (x : P) :
     perm_kind (perm_unlock x) ≠ Locked;
-  perm_assoc :> Associative (=) (∪);
-  perm_comm :> Commutative (=) (∪);
-  perm_disjoint_union_ll x y z :
+  perm_assoc :> Associative (=) (@union P _);
+  perm_comm :> Commutative (=) (@union P _);
+  perm_disjoint_union_ll (x y z : P) :
     x ∪ y ⊥ z → x ⊥ z;
-  perm_disjoint_union_move_l x y z :
+  perm_disjoint_union_move_l (x y z : P) :
     x ∪ y ⊥ z → x ⊥ y ∪ z;
-  perm_union_subset_l x y :
+  perm_union_subset_l (x y : P) :
     x ⊥ y →
     x ⊂ x ∪ y;
-  perm_union_preserving_l x y z :
+  perm_union_preserving_l (x y z : P) :
     x ⊆ y → z ∪ x ⊆ z ∪ y;
-  perm_union_reflecting_l x y z :
+  perm_union_reflecting_l (x y z : P) :
     z ⊥ x → z ⊥ y →
     z ∪ x ⊆ z ∪ y →
     x ⊆ y;
-  perm_difference_disjoint x y :
+  perm_difference_disjoint (x y : P) :
     x ⊂ y → x ⊥ y ∖ x;
-  perm_union_difference x y :
+  perm_union_difference (x y : P) :
     x ⊂ y →
     x ∪ y ∖ x = y
 }.
 
-(** * General properties of permissions *)
+Class FracPermissions (P : Set) `{PermissionsOps P} `{Half P} : Prop := {
+  frac_permissions :> Permissions P;
+  perm_disjoint_half (x : P) :
+    perm_kind x ≠ Locked →
+    x.½ ⊥ x.½;
+  perm_union_half (x : P) :
+    x.½ ∪ x.½ = x
+}.
+
+(** * General properties of fractional permissions *)
 (** We prove some derived properties for arbitrary permission implementations.
 Many of these properties are just variants of the laws using commutativity of
 [(∪)] and symmetry of [(⊥)]. *)
 Section permissions.
 Context `{Permissions P}.
 
-Lemma perm_disjoint_kind_l x y : x ⊥ y → perm_kind x = Read.
+Lemma perm_fragment_alt (x : P) :
+  perm_fragment x ↔ ∃ y, x ⊂ y.
+Proof.
+  split.
+  * intros [y ?]. exists (x ∪ y). eauto using perm_union_subset_l.
+  * intros [y ?]. exists (y ∖ x). eauto using perm_difference_disjoint.
+Qed.
+
+Lemma perm_disjoint_kind_l (x y : P) : x ⊥ y → perm_kind x = Read.
 Proof. intros. apply perm_fragment_read. by exists y. Qed.
-Lemma perm_disjoint_kind_r x y : x ⊥ y → perm_kind y = Read.
+Lemma perm_disjoint_kind_r (x y : P) :  x ⊥ y → perm_kind y = Read.
 Proof. intros. by apply perm_disjoint_kind_l with x. Qed.
-Lemma perm_disjoint_locked_l x y : x ⊥ y → perm_kind x ≠ Locked.
+Lemma perm_disjoint_locked_l (x y : P) :  x ⊥ y → perm_kind x ≠ Locked.
 Proof. intros Hxy ?. apply perm_disjoint_kind_l in Hxy. congruence. Qed.
-Lemma perm_disjoint_locked_r x y : x ⊥ y → perm_kind y ≠ Locked.
+Lemma perm_disjoint_locked_r (x y : P) :  x ⊥ y → perm_kind y ≠ Locked.
 Proof. intros Hxy ?. apply perm_disjoint_kind_r in Hxy. congruence. Qed.
-Lemma perm_disjoint_write_l x y : x ⊥ y → perm_kind x ≠ Write.
+Lemma perm_disjoint_write_l (x y : P) :  x ⊥ y → perm_kind x ≠ Write.
 Proof. intros Hxy ?. apply perm_disjoint_kind_l in Hxy. congruence. Qed.
-Lemma perm_disjoint_write_r x y : x ⊥ y → perm_kind y ≠ Write.
+Lemma perm_disjoint_write_r (x y : P) :  x ⊥ y → perm_kind y ≠ Write.
 Proof. intros Hxy ?. apply perm_disjoint_kind_r in Hxy. congruence. Qed.
-Lemma perm_disjoint_free_l x y : x ⊥ y → perm_kind x ≠ Free.
+Lemma perm_disjoint_free_l (x y : P) :  x ⊥ y → perm_kind x ≠ Free.
 Proof. intros Hxy ?. apply perm_disjoint_kind_l in Hxy. congruence. Qed.
-Lemma perm_disjoint_free_r x y : x ⊥ y → perm_kind y ≠ Free.
+Lemma perm_disjoint_free_r (x y : P) :  x ⊥ y → perm_kind y ≠ Free.
 Proof. intros Hxy ?. apply perm_disjoint_kind_r in Hxy. congruence. Qed.
 
-Lemma perm_fragment_not_read x : perm_kind x ≠ Read → ¬perm_fragment x.
+Lemma perm_fragment_not_read (x : P) :  perm_kind x ≠ Read → ¬perm_fragment x.
 Proof. intuition auto using perm_fragment_read. Qed.
-Lemma perm_fragment_write x : perm_kind x = Write → ¬perm_fragment x.
+Lemma perm_fragment_write (x : P) :  perm_kind x = Write → ¬perm_fragment x.
 Proof. intros ? Hx. apply perm_fragment_read in Hx. congruence. Qed.
-Lemma perm_fragment_free x : perm_kind x = Free → ¬perm_fragment x.
+Lemma perm_fragment_free (x : P) :  perm_kind x = Free → ¬perm_fragment x.
 Proof. intros ? Hx. apply perm_fragment_read in Hx. congruence. Qed.
-Lemma perm_fragment_subseteq_write x :
+Lemma perm_fragment_subseteq_write (x : P) :
   Write ⊆ perm_kind x → ¬perm_fragment x.
 Proof.
   rewrite Write_subseteq.
   intros [?|?]; eauto using perm_fragment_write, perm_fragment_free.
 Qed.
-Lemma perm_fragment_locked x : perm_kind x = Locked → ¬perm_fragment x.
+Lemma perm_fragment_locked (x : P) :  perm_kind x = Locked → ¬perm_fragment x.
 Proof. intros ? Hx. apply perm_fragment_read in Hx. congruence. Qed.
 
-Lemma perm_disjoint_weaken_r x y y' :
+Lemma perm_disjoint_weaken_r (x y y' : P) :
   x ⊥ y → y' ⊆ y → x ⊥ y'.
 Proof. rewrite !(symmetry_iff _ x). apply perm_disjoint_weaken_l. Qed.
-Lemma perm_disjoint_weaken x x' y y' :
+Lemma perm_disjoint_weaken (x x' y y' : P) :
   x ⊥ y → x' ⊆ x → y' ⊆ y → x' ⊥ y'.
 Proof. eauto using perm_disjoint_weaken_l, perm_disjoint_weaken_r. Qed.
 
-Lemma perm_disjoint_union_lr x y z :
+Lemma perm_disjoint_union_lr (x y z : P) :
   x ∪ y ⊥ z → y ⊥ z.
 Proof. rewrite (commutative _). apply perm_disjoint_union_ll. Qed.
-Lemma perm_disjoint_union_rl x y z :
+Lemma perm_disjoint_union_rl (x y z : P) :
   x ⊥ y ∪ z → x ⊥ y.
 Proof. rewrite !(symmetry_iff _ x). apply perm_disjoint_union_ll. Qed.
-Lemma perm_disjoint_union_rr x y z :
+Lemma perm_disjoint_union_rr (x y z : P) :
   x ⊥ y ∪ z → x ⊥ z.
 Proof. rewrite (commutative _). apply perm_disjoint_union_rl. Qed.
 
-Lemma perm_disjoint_union_move_r x y z :
+Lemma perm_disjoint_union_move_r (x y z : P) :
   x ⊥ y ∪ z → x ∪ y ⊥ z.
 Proof.
   intros. symmetry. rewrite (commutative _).
   apply perm_disjoint_union_move_l. by rewrite (commutative _).
 Qed.
 
-Lemma perm_disjoint_union_l x y z :
+Lemma perm_disjoint_union_l (x y z : P) :
   x ∪ y ⊥ z → x ⊥ y.
 Proof. eauto using perm_disjoint_union_rl, perm_disjoint_union_move_l. Qed.
-Lemma perm_disjoint_union_r x y z :
+Lemma perm_disjoint_union_r (x y z : P) :
   x ⊥ y ∪ z → y ⊥ z.
 Proof. eauto using perm_disjoint_union_lr, perm_disjoint_union_move_r. Qed.
 
-Lemma perm_union_subset_r x y :
+Lemma perm_union_subset_r (x y : P) :
   y ⊥ x → x ⊂ y ∪ x.
 Proof.
   rewrite (symmetry_iff _), (commutative_eq (∪)).
   by apply perm_union_subset_l.
 Qed.
-Lemma perm_union_subseteq_l x y :
+Lemma perm_union_subseteq_l (x y : P) :
   x ⊥ y → x ⊆ x ∪ y.
 Proof. intros. by apply subset_subseteq, perm_union_subset_l. Qed.
-Lemma perm_union_subseteq_r x y :
+Lemma perm_union_subseteq_r (x y : P) :
   y ⊥ x → x ⊆ y ∪ x.
 Proof. intros. by apply subset_subseteq, perm_union_subset_r. Qed.
-Lemma perm_union_ne_l x y :
+Lemma perm_union_ne_l (x y : P) :
   x ⊥ y → x ≠ x ∪ y.
 Proof.
   intros ? E. destruct (perm_union_subset_l x y) as [? []]; auto.
   by rewrite <-E.
 Qed.
-Lemma perm_union_ne_r x y :
+Lemma perm_union_ne_r (x y : P) :
   y ⊥ x → x ≠ y ∪ x.
 Proof.
   intros ? E. destruct (perm_union_subset_r x y) as [? []]; auto.
   by rewrite <-E.
 Qed.
 
-Lemma perm_union_preserving_r x y z :
+Lemma perm_union_preserving_r (x y z : P) :
   x ⊆ y → x ∪ z ⊆ y ∪ z.
 Proof. rewrite !(commutative _ _ z). apply perm_union_preserving_l. Qed.
-Lemma perm_union_strict_preserving_l x y z :
+Lemma perm_union_strict_preserving_l (x y z : P) :
   z ⊥ x → z ⊥ y →
   x ⊂ y → z ∪ x ⊂ z ∪ y.
 Proof.
@@ -278,7 +299,7 @@ Proof.
   * auto using perm_union_preserving_l.
   * contradict Hxy2. by apply perm_union_reflecting_l with z.
 Qed.
-Lemma perm_union_strict_preserving_r x y z :
+Lemma perm_union_strict_preserving_r (x y z : P) :
   x ⊥ z → y ⊥ z →
   x ⊂ y → x ∪ z ⊂ y ∪ z.
 Proof.
@@ -286,14 +307,14 @@ Proof.
   by apply perm_union_strict_preserving_l.
 Qed.
 
-Lemma perm_union_reflecting_r x y z :
+Lemma perm_union_reflecting_r (x y z : P) :
   x ⊥ z → y ⊥ z →
   x ∪ z ⊆ y ∪ z → x ⊆ y.
 Proof.
   intros ??. rewrite !(commutative_eq (∪) _ z).
   by apply perm_union_reflecting_l.
 Qed.
-Lemma perm_union_strict_reflecting_l x y z :
+Lemma perm_union_strict_reflecting_l (x y z : P) :
   z ⊥ x → z ⊥ y →
   z ∪ x ⊂ z ∪ y → x ⊂ y.
 Proof.
@@ -301,7 +322,7 @@ Proof.
   * eauto using perm_union_reflecting_l.
   * contradict Hxy2. by apply perm_union_preserving_l.
 Qed.
-Lemma perm_union_strict_reflecting_r x y z :
+Lemma perm_union_strict_reflecting_r (x y z : P) :
   x ⊥ z → y ⊥ z →
   x ∪ z ⊂ y ∪ z → x ⊂ y.
 Proof.
@@ -309,14 +330,14 @@ Proof.
   apply perm_union_strict_reflecting_l.
 Qed.
 
-Lemma perm_union_cancel_l x y z :
+Lemma perm_union_cancel_l (x y z : P) :
   z ⊥ x → z ⊥ y →
   z ∪ x = z ∪ y → x = y.
 Proof.
   intros ?? E. by apply (anti_symmetric _);
     apply perm_union_reflecting_l with z; rewrite ?E.
 Qed.
-Lemma perm_union_cancel_r x y z :
+Lemma perm_union_cancel_r (x y z : P) :
   x ⊥ z → y ⊥ z →
   x ∪ z = y ∪ z → x = y.
 Proof.
@@ -324,38 +345,66 @@ Proof.
   by apply perm_union_cancel_l.
 Qed.
 
-Lemma perm_kind_union x y :
+Lemma perm_kind_union_l (x y : P) :
+  x ⊥ y →
+  perm_kind x ⊆ perm_kind (x ∪ y).
+Proof. intros. by apply perm_kind_preserving, perm_union_subseteq_l. Qed.
+Lemma perm_kind_union_r (x y : P) :
+  x ⊥ y →
+  perm_kind y ⊆ perm_kind (x ∪ y).
+Proof. intros. by apply perm_kind_preserving, perm_union_subseteq_r. Qed.
+Lemma perm_kind_union_locked (x y : P) :
   x ⊥ y →
   perm_kind (x ∪ y) ≠ Locked.
 Proof.
-  intros ? Hxy. feed pose proof (perm_kind_preserving x (x ∪ y))
-    as Hxxy; auto using perm_union_subseteq_l.
+  intros Hdisjoint Hxy. pose proof (perm_kind_union_l x y Hdisjoint) as Hxxy.
   rewrite (perm_disjoint_kind_l x y), Hxy in Hxxy by done.
   by inversion Hxxy.
 Qed.
 
-Lemma perm_unlock_union x y :
+Lemma perm_unlock_union (x y : P) :
   x ⊥ y →
   perm_unlock (x ∪ y) = perm_unlock x ∪ perm_unlock y.
 Proof.
-  intros. by rewrite !perm_unlock_other by eauto using perm_kind_union,
+  intros. by rewrite !perm_unlock_other by eauto using perm_kind_union_locked,
      perm_disjoint_locked_l, perm_disjoint_locked_r.
 Qed.
 
-Lemma perm_disjoint_unlock_l x y :
+Lemma perm_disjoint_unlock_l (x y : P) :
   x ⊥ y → perm_unlock x ⊥ y.
 Proof.
   destruct (decide (perm_kind x = Locked)).
   * intros. by destruct (perm_disjoint_locked_l x y).
   * by rewrite perm_unlock_other.
 Qed.
-Lemma perm_disjoint_unlock_r x y :
+Lemma perm_disjoint_unlock_r (x y : P) :
   x ⊥ y → x ⊥ perm_unlock y.
 Proof. intros. symmetry. by apply perm_disjoint_unlock_l. Qed.
 
-Lemma perm_unlock_idempotent x :
+Lemma perm_unlock_idempotent (x : P) :
   perm_unlock (perm_unlock x) = perm_unlock x.
 Proof.
   rewrite (perm_unlock_other (perm_unlock x)); auto using perm_unlock_kind.
 Qed.
 End permissions.
+
+Section frac_permissions.
+Context `{FracPermissions P}.
+
+Lemma perm_half_subseteq (x : P) :
+  perm_kind x ≠ Locked →
+  x.½ ⊆ x.
+Proof.
+  intros. rewrite <-(perm_union_half x) at 2.
+  by apply perm_union_subseteq_l, perm_disjoint_half.
+Qed.
+
+Lemma perm_kind_half (x : P) :
+  perm_kind x ≠ Locked →
+  perm_kind (x.½) = Read.
+Proof. intros. by eapply perm_disjoint_kind_l, perm_disjoint_half. Qed.
+Lemma perm_kind_half_locked (x : P) :
+  perm_kind x ≠ Locked →
+  perm_kind (x.½) ≠ Locked.
+Proof. intros Hx. apply perm_kind_half in Hx. congruence. Qed.
+End frac_permissions.
