frac.v
@@ -14,8 +14,6 @@ Require Export abstract_permissions numbers.
 Local Open Scope Qc_scope.
 
 Definition frac : Set := dsigS (λ x : Qc, 0 < x ≤ 1).
-Bind Scope frac_scope with frac.
-Delimit Scope frac_scope with frac.
 
 Definition frac_bounds (f : frac) : 0 < `f ≤ 1 := proj2_dsig f.
 Lemma frac_lower (f : frac) : 0 < `f.
@@ -25,42 +23,29 @@ Proof. apply frac_bounds. Qed.
 
 Program Definition frac1 : frac := dexist 1%Qc _.
 Next Obligation. done. Qed.
-Notation "1" := frac1 : frac_scope.
 
 Definition frac_gen_kind (k : pkind) (f : frac) : pkind :=
-  if decide (f = 1%frac) then k else Read.
-Instance frac_kind: PermKind frac := frac_gen_kind Write.
+  if decide (f = frac1) then k else Read.
 
-Instance frac_lock: PermLock frac := λ _ f, f.
-
-Instance frac_subseteq: SubsetEq frac := λ f1 f2, `f1 ≤ `f2.
-Instance frac_subseteq_dec (f1 f2 : frac) :
-  Decision (f1 ⊆ f2) := decide (`f1 ≤ `f2).
-
-Lemma frac_subset_spec f1 f2 : f1 ⊂ f2 ↔ `f1 < `f2.
-Proof.
-  unfold subset, orders.preorder_subset, subseteq, frac_subseteq.
-  rewrite <-Qclt_nge. intuition auto using Qclt_le_weak.
-Qed.
-
-Instance frac_disjoint: Disjoint frac := λ f1 f2, `f1 + `f2 ≤ 1.
-Instance frac_disjoint_dec (f1 f2 : frac) :
-  Decision (f1 ⊥ f2) := decide (`f1 + `f2 ≤ 1).
-
-Program Instance frac_union: Union frac := λ f1 f2,
-  if decide (`f1 + `f2 ≤ 1)
-  then dexist (`f1 + `f2) _
-  else 1%frac (**i dummy *).
+Program Instance frac_ops: PermissionsOps frac := {
+  perm_kind := frac_gen_kind Write;
+  perm_lock_ := λ _ f, f;
+  perm_subseteq := λ f1 f2, `f1 ≤ `f2;
+  perm_disjoint := λ f1 f2, `f1 + `f2 ≤ 1;
+  perm_union := λ f1 f2,
+    if decide (`f1 + `f2 ≤ 1)
+    then dexist (`f1 + `f2) _
+    else frac1;
+  perm_difference := λ f1 f2,
+    if decide (`f2 < `f1)
+    then dexist (`f1 - `f2) _
+    else frac1 (**i dummy *)
+}.
 Next Obligation.
   split; [|done]. apply Qclt_le_trans with (`f1 + 0).
   * ring_simplify. auto using frac_lower.
   * rewrite <-Qcplus_le_mono_l. auto using Qclt_le_weak, frac_lower.
 Qed.
-
-Program Instance frac_difference: Difference frac := λ f1 f2,
-  if decide (`f2 < `f1)
-  then dexist (`f1 - `f2) _
-  else 1%frac (**i dummy *).
 Next Obligation.
   unfold Qcminus. split.
   { by rewrite <-Qclt_minus_iff. }
@@ -68,6 +53,12 @@ Next Obligation.
   * rewrite <-Qcplus_le_mono_l.
     apply (Qcopp_le_compat 0 (`f2)), Qclt_le_weak, frac_lower.
   * rewrite Qcplus_0_r. apply frac_upper.
+Qed.
+
+Lemma frac_subset_spec f1 f2 : f1 ⊂ f2 ↔ `f1 < `f2.
+Proof.
+  unfold subset, orders.preorder_subset, subseteq, perm_subseteq; simpl.
+  rewrite <-Qclt_nge. intuition auto using Qclt_le_weak.
 Qed.
 
 Local Instance: PartialOrder frac.
@@ -79,28 +70,28 @@ Proof.
 Qed.
 Local Instance: Symmetric (@disjoint frac _).
 Proof.
-  intros ??. unfold disjoint, frac_disjoint.
+  intros ??. unfold disjoint, perm_disjoint; simpl.
   by rewrite Qcplus_comm.
 Qed.
 
-Lemma frac_disjoint_weaken_l f1 f1' f2 :
+Lemma frac_disjoint_weaken_l (f1 f1' f2 : frac) :
   f1 ⊥ f2 →
   f1' ⊆ f1 →
   f1' ⊥ f2.
 Proof.
-  unfold disjoint, frac_disjoint, subseteq, frac_subseteq.
+  unfold disjoint, perm_disjoint, subseteq, perm_subseteq; simpl.
   intros ??. transitivity (`f1 + `f2); [|done].
   by apply Qcplus_le_mono_r.
 Qed.
 
-Lemma frac_union_not_disjoint f1 f2 :
+Lemma frac_union_not_disjoint (f1 f2 : frac) :
   ¬f1 ⊥ f2 →
-  f1 ∪ f2 = 1%frac.
-Proof. intros. unfold union, frac_union. by case_decide. Qed.
-Lemma frac_union_disjoint f1 f2 :
+  f1 ∪ f2 = frac1.
+Proof. intros. unfold union, perm_union; simpl. by case_decide. Qed.
+Lemma frac_union_disjoint (f1 f2 : frac) :
   f1 ⊥ f2 →
   @proj1_sig Qc _ (f1 ∪ f2) = `f1 + `f2.
-Proof. intros. unfold union, frac_union. by case_decide. Qed.
+Proof. intros. unfold union, perm_union; simpl. by case_decide. Qed.
 
 Local Instance: Commutative (=) (@union frac _).
 Proof.
@@ -110,10 +101,10 @@ Proof.
   * by rewrite !frac_union_not_disjoint.
 Qed.
 
-Lemma frac_disjoint_union_ll f1 f2 f3 :
+Lemma frac_disjoint_union_ll (f1 f2 f3 : frac) :
   f1 ∪ f2 ⊥ f3 → f1 ⊥ f3.
 Proof.
-  unfold union, frac_union, disjoint, frac_disjoint; simpl.
+  unfold union, perm_union, disjoint, perm_disjoint; simpl.
   case_decide; simpl.
   * intros. transitivity (`f1 + `f2 + `f3); [|done].
     replace (`f1 + `f3) with (0 + (`f1 + `f3)) by ring.
@@ -122,56 +113,56 @@ Proof.
   * rewrite Qcle_ngt. intros [].
     apply (Qcplus_lt_mono_l 0 (`f3) 1), frac_lower.
 Qed.
-Lemma frac_disjoint_union_lr f1 f2 f3 :
+Lemma frac_disjoint_union_lr (f1 f2 f3 : frac) :
   f1 ∪ f2 ⊥ f3 → f2 ⊥ f3.
 Proof. rewrite (commutative (∪)). apply frac_disjoint_union_ll. Qed.
-Lemma frac_disjoint_union_rl f1 f2 f3 :
+Lemma frac_disjoint_union_rl (f1 f2 f3 : frac) :
   f1 ⊥ f2 ∪ f3 → f1 ⊥ f2.
 Proof. rewrite !(symmetry_iff (⊥) f1). apply frac_disjoint_union_ll. Qed.
-Lemma frac_disjoint_union_rr f1 f2 f3 :
+Lemma frac_disjoint_union_rr (f1 f2 f3 : frac) :
   f1 ⊥ f2 ∪ f3 → f1 ⊥ f3.
 Proof. rewrite (commutative (∪)). apply frac_disjoint_union_rl. Qed.
 
-Lemma frac_disjoint_union_l f1 f2 f3 :
+Lemma frac_disjoint_union_l (f1 f2 f3 : frac) :
   f1 ∪ f2 ⊥ f3 → f1 ⊥ f2.
 Proof.
   intros H1. apply dec_stable.
-  unfold disjoint, frac_disjoint in H1.
+  unfold disjoint, perm_disjoint in H1; simpl in H1.
   rewrite Qcle_ngt in H1. contradict H1.
   rewrite frac_union_not_disjoint by done.
   apply (Qcplus_lt_mono_l 0 (`f3) 1), frac_lower.
 Qed.
 
-Lemma frac_disjoint_union_move_l f1 f2 f3 :
+Lemma frac_disjoint_union_move_l (f1 f2 f3 : frac) :
   f1 ∪ f2 ⊥ f3 → f1 ⊥ f2 ∪ f3.
 Proof.
   intros H1. pose proof (frac_disjoint_union_l _ _ _ H1).
-  unfold disjoint, frac_disjoint.
+  unfold disjoint, perm_disjoint; simpl.
   rewrite frac_union_disjoint, Qcplus_assoc by
     (by apply frac_disjoint_union_lr with f1).
-  unfold disjoint, frac_disjoint in H1.
+  unfold disjoint, perm_disjoint in H1; simpl in H1.
   by rewrite frac_union_disjoint in H1.
 Qed.
-Lemma frac_disjoint_union_move_r f1 f2 f3 :
+Lemma frac_disjoint_union_move_r (f1 f2 f3 : frac) :
   f1 ⊥ f2 ∪ f3 → f1 ∪ f2 ⊥ f3.
 Proof.
   intros. symmetry. rewrite (commutative _).
   apply frac_disjoint_union_move_l. by rewrite (commutative _).
 Qed.
 
-Lemma frac_1_max f : f ⊆ 1%frac.
+Lemma frac_1_max f : f ⊆ frac1.
 Proof. apply frac_upper. Qed.
 Lemma frac_1_max_alt f :
-  1%frac ⊆ f → f = 1%frac.
+  frac1 ⊆ f → f = frac1.
 Proof. intros. apply (anti_symmetric _); auto using frac_1_max. Qed.
 
-Lemma frac_disjoint_1_l f : ¬1%frac ⊥ f.
+Lemma frac_disjoint_1_l f : ¬frac1 ⊥ f.
 Proof.
-  unfold disjoint, frac_disjoint. simpl. intros H.
+  unfold disjoint, perm_disjoint; simpl. intros H.
   apply (Qcle_not_lt (`f) 0); auto using frac_lower.
   by rewrite (Qcplus_le_mono_l _ _ 1).
 Qed.
-Lemma frac_disjoint_1_r f : ¬f ⊥ 1%frac.
+Lemma frac_disjoint_1_r f : ¬f ⊥ frac1.
 Proof. rewrite (symmetry_iff _). by apply frac_disjoint_1_l. Qed.
 
 Lemma frac_gen_kind_preserving k f1 f2 :
@@ -195,7 +186,7 @@ Lemma frac_unlock_kind k f :
   frac_gen_kind k (perm_unlock f) ≠ Locked.
 Proof. unfold frac_gen_kind. by case_decide. Qed.
 
-Instance: Permissions frac.
+Local Instance: Permissions frac.
 Proof.
   split.
   * apply _.
@@ -222,7 +213,7 @@ Proof.
     rewrite frac_union_disjoint by done.
     rewrite <-(Qcplus_0_r (`f1)) at 1.
     apply Qcplus_lt_mono_l, frac_lower.
-  * intros f1 f2 f3 H1. unfold subseteq, frac_subseteq.
+  * intros f1 f2 f3 H1. unfold subseteq, perm_subseteq; simpl.
     destruct (decide (f3 ⊥ f2)).
     + assert (f3 ⊥ f1).
       { symmetry. by apply frac_disjoint_weaken_l with f2. }
@@ -232,47 +223,51 @@ Proof.
       destruct (decide (f3 ⊥ f1)).
       { by rewrite frac_union_disjoint. }
       by rewrite frac_union_not_disjoint.
-  * intros f1 f2 f3 H1 H2 H3. unfold subseteq, frac_subseteq in *.
+  * intros f1 f2 f3 H1 H2 H3. unfold subseteq, perm_subseteq in *; simpl in *.
     rewrite !frac_union_disjoint in H3 by done.
     by rewrite (Qcplus_le_mono_l _ _ (`f3)).
   * intros f1 f2 H1. do 2 red. rewrite frac_subset_spec in H1.
-    unfold difference, frac_difference. case_decide; simpl; [|done].
+    unfold difference, perm_difference; simpl. case_decide; simpl; [|done].
     transitivity (`f1 + (`f2 - `f1)).
     { by rewrite <-Qcplus_le_mono_r. }
     replace (`f1 + (`f2 - `f1)) with (`f2) by ring. apply frac_upper.
   * intros f1 f2 H1. rewrite frac_subset_spec in H1. apply dsig_eq.
-    unfold difference, frac_difference. case_decide; simpl; [|done].
-    unfold union, frac_union. case_decide; simpl. ring.
+    unfold difference, perm_difference; simpl. case_decide; simpl; [|done].
+    unfold union, perm_union; simpl. case_decide; simpl. ring.
     assert (`f1 + (`f2 - `f1) ≤ 1); [|done].
     ring_simplify. apply frac_upper.
 Qed.
 
-Instance: LeftAbsorb (=) 1%frac (∪).
+Instance: LeftAbsorb (=) frac1 (∪).
 Proof.
   intros ?. apply dsig_eq.
   rewrite frac_union_not_disjoint; eauto using frac_disjoint_1_l.
 Qed.
-Instance: RightAbsorb (=) 1%frac (∪).
+Instance: RightAbsorb (=) frac1 (∪).
 Proof. intro. rewrite (commutative_eq (∪)). apply (left_absorb _ _). Qed.
 
-Program Definition frac_split (f : frac) : frac := dexist (`f / 2) _.
+Program Instance frac_half: Half frac := λ f, dexist (`f / 2) _.
 Next Obligation.
   split.
   * by apply (Qcmult_lt_compat_r 0 (`f) (/2)); auto using frac_lower.
   * apply (Qcmult_le_compat_r (`f) 2 (/2)); [|done].
     by transitivity 1; auto using frac_upper.
 Qed.
-Notation "f ↓" := (frac_split f) (at level 20) : frac_scope.
 
-Lemma frac_split_disjoint f : (f↓ ⊥ f↓)%frac.
+Lemma frac_disjoint_half (f : frac) : f.½ ⊥ f.½.
 Proof.
   change (`f * /2 + `f * /2 ≤ 1). rewrite <-Qcmult_plus_distr_r.
   replace (/2 + /2) with 1 by (by apply Qc_is_canon).
   rewrite Qcmult_1_r. apply frac_upper.
 Qed.
-Lemma frac_split_union f : (f↓ ∪ f↓ = f)%frac.
+
+Instance: FracPermissions frac.
 Proof.
-  apply dsig_eq. rewrite frac_union_disjoint by auto using frac_split_disjoint.
-  simpl. unfold Qcdiv. rewrite <-Qcmult_plus_distr_r.
-  replace (/2 + /2) with 1 by (by apply Qc_is_canon). ring.
+  split.
+  * apply _.
+  * intros. apply frac_disjoint_half.
+  * intros f. apply dsig_eq.
+    rewrite frac_union_disjoint by auto using frac_disjoint_half.
+    simpl. unfold Qcdiv. rewrite <-Qcmult_plus_distr_r.
+    replace (/2 + /2) with 1 by (by apply Qc_is_canon). ring.
 Qed.
