seqfrac.v
@@ -12,20 +12,54 @@ Definition seqfrac_gen_kind (k : pkind) (f : seqfrac) : pkind :=
   | Seq => Locked
   | UnSeq f => frac_gen_kind k f
   end.
-Instance seqfrac_kind: PermKind seqfrac := seqfrac_gen_kind Write.
 
-Instance seqfrac_lock: PermLock seqfrac := λ l f,
-  match l, f with
-  | true, _ => Seq
-  | false, Seq => UnSeq 1
-  | false, UnSeq f => UnSeq f
-  end.
 Inductive seqfrac_subseteq: SubsetEq seqfrac :=
   | Seq_subseteq_Seq :
      Seq ⊆ Seq
   | UnSeq_subseteq_UnSeq f1 f2 :
      f1 ⊆ f2 → UnSeq f1 ⊆ UnSeq f2.
-Existing Instance seqfrac_subseteq.
+Inductive seqfrac_disjoint: Disjoint seqfrac :=
+  | UnSeq_disjoint f1 f2 :
+     f1 ⊥ f2 → UnSeq f1 ⊥ UnSeq f2.
+
+Instance seqfrac_ops: PermissionsOps seqfrac := {
+  perm_kind := seqfrac_gen_kind Write;
+  perm_lock_ := λ l f,
+    match l, f with
+    | true, _ => Seq
+    | false, Seq => UnSeq frac1
+    | false, UnSeq f => UnSeq f
+    end;
+  perm_subseteq := seqfrac_subseteq;
+  perm_disjoint := seqfrac_disjoint;
+  perm_union := λ f1 f2,
+    match f1, f2 with
+    | UnSeq f1, UnSeq f2 => UnSeq (f1 ∪ f2)
+    | _, _ => Seq (**i dummy *)
+    end;
+  perm_difference := λ f1 f2,
+    match f1, f2 with
+    | UnSeq f1, UnSeq f2 => UnSeq (f1 ∖ f2)
+    | _, _ => Seq (**i dummy *)
+    end;
+  perm_disjoint_dec := λ f1 f2, _;
+  perm_eq_dec := λ f1 f2, _;
+  perm_subseteq_dec := λ f1 f2, _
+}.
+Proof.
+ refine
+  match f1, f2 with
+  | UnSeq f1, UnSeq f2 => cast_if (decide (f1 ⊥ f2))
+  | _, _ => right _
+  end; first [by constructor | by inversion 1].
+ solve_decision.
+ refine
+  match f1, f2 with
+  | Seq, Seq => left _
+  | UnSeq f1, UnSeq f2 => cast_if (decide (f1 ⊆ f2))
+  | _, _ => right _
+  end; first [by subst; constructor | by inversion 1; subst].
+Defined.
 
 Lemma UnSeq_subset_UnSeq f1 f2 : f1 ⊂ f2 → UnSeq f1 ⊂ UnSeq f2.
 Proof. intros [? H]. by split; [constructor|contradict H; inversion H]. Qed.
@@ -40,43 +74,6 @@ Proof.
     + repeat esplit; eauto. contradict H2. by constructor.
   * naive_solver eauto using UnSeq_subset_UnSeq.
 Qed.
-
-Inductive seqfrac_disjoint: Disjoint seqfrac :=
-  | UnSeq_disjoint f1 f2 :
-     f1 ⊥ f2 → UnSeq f1 ⊥ UnSeq f2.
-Existing Instance seqfrac_disjoint.
-
-Instance seqfrac_union: Union seqfrac := λ f1 f2,
-  match f1, f2 with
-  | UnSeq f1, UnSeq f2 => UnSeq (f1 ∪ f2)
-  | _, _ => Seq (**i dummy *)
-  end.
-
-Instance seqfrac_difference: Difference seqfrac := λ f1 f2,
-  match f1, f2 with
-  | UnSeq f1, UnSeq f2 => UnSeq (f1 ∖ f2)
-  | _, _ => Seq (**i dummy *)
-  end.
-
-Instance seqfrac_eq_dec (f1 f2 : seqfrac) : Decision (f1 = f2).
-Proof. solve_decision. Defined.
-Instance seqfrac_subseteq_dec (f1 f2 : seqfrac) : Decision (f1 ⊆ f2).
-Proof.
- refine
-  match f1, f2 with
-  | Seq, Seq => left _
-  | UnSeq f1, UnSeq f2 => cast_if (decide (f1 ⊆ f2))
-  | _, _ => right _
-  end; first [by subst; constructor | by inversion 1; subst].
-Defined.
-Instance seqfrac_disjoint_dec (f1 f2 : seqfrac) : Decision (f1 ⊥ f2).
-Proof.
- refine
-  match f1, f2 with
-  | UnSeq f1, UnSeq f2 => cast_if (decide (f1 ⊥ f2))
-  | _, _ => right _
-  end; first [by constructor | by inversion 1].
-Defined.
 
 Lemma seqfrac_gen_kind_preserving k f1 f2 :
   Read ⊆ k →
@@ -99,7 +96,7 @@ Lemma seqfrac_lock_unlock k f :
   seqfrac_gen_kind k f = Locked →
   perm_lock (perm_unlock f) = f.
 Proof.
-  unfold perm_lock_, seqfrac_lock. destruct f; simpl.
+  unfold perm_lock_; destruct f; simpl.
   * done.
   * unfold frac_gen_kind. case_decide. by inversion 1; subst. done.
 Qed.
@@ -107,7 +104,7 @@ Lemma seqfrac_unlock_lock k f :
   Write ⊆ seqfrac_gen_kind k f →
   perm_unlock (perm_lock f) = f.
 Proof.
-  unfold perm_lock_, seqfrac_lock. destruct f; simpl.
+  unfold perm_lock_; destruct f; simpl.
   * inversion 1.
   * unfold frac_gen_kind. case_decide. by subst. inversion 1.
 Qed.
@@ -139,28 +136,28 @@ Proof.
   * apply seqfrac_unlock_lock.
   * apply seqfrac_unlock_other.
   * intros. by apply seqfrac_unlock_kind.
-  * red. unfold union, seqfrac_union.
+  * red. unfold union, perm_union. simpl.
     intros [|?] [|?] [|?]; try reflexivity.
     f_equal. apply (associative_eq _).
-  * red. unfold union, seqfrac_union.
+  * red. unfold union, perm_union; simpl.
     intros [|?] [|?]; try reflexivity. f_equal. apply (commutative _).
-  * unfold union, seqfrac_union.
+  * unfold union, perm_union; simpl.
     intros [|?] [|?]; inversion_clear 1.
     constructor. eapply perm_disjoint_union_ll; eauto.
-  * unfold union, seqfrac_union.
+  * unfold union, perm_union; simpl.
     intros [|?] [|?]; inversion_clear 1.
     constructor. by apply perm_disjoint_union_move_l.
-  * unfold union, seqfrac_union. destruct 1.
+  * unfold union, perm_union; simpl. destruct 1.
     by apply UnSeq_subset_UnSeq, perm_union_subset_l.
-  * unfold union, seqfrac_union.
+  * unfold union, perm_union; simpl.
     intros ?? [|?]; destruct 1; try constructor.
     by apply perm_union_preserving_l.
   * destruct 1; inversion 1; inversion 1.
     constructor. eapply perm_union_reflecting_l; eauto.
-  * unfold union, difference, seqfrac_union, seqfrac_difference.
+  * unfold union, difference, perm_union, perm_difference; simpl.
     intros ??. rewrite seqfrac_subset_alt. intros (?&?&?&?&?); subst.
     constructor; by apply perm_difference_disjoint.
-  * unfold union, difference, seqfrac_union, seqfrac_difference.
+  * unfold union, difference, perm_union, perm_difference; simpl.
     intros ??. rewrite seqfrac_subset_alt. intros (?&?&?&?&?); subst.
     f_equal. by apply perm_union_difference.
 Qed.
@@ -181,6 +178,25 @@ Proof. intros [? H]. inversion H. Qed.
 
 Definition to_frac (f : seqfrac) : frac :=
   match f with
-  | Seq => 1%frac
+  | Seq => frac1
   | UnSeq f => f
   end.
+
+Instance seqfrac_half: Half seqfrac := λ f,
+  match f with
+  | Seq => Seq
+  | UnSeq f => UnSeq (f.½)
+  end.
+Lemma seqfrac_disjoint_half k f :
+  seqfrac_gen_kind k f ≠ Locked →
+  f.½ ⊥ f.½.
+Proof. destruct f; [done |]. constructor. apply frac_disjoint_half. Qed.
+
+Instance: FracPermissions seqfrac.
+Proof.
+  split.
+  * apply _.
+  * apply seqfrac_disjoint_half.
+  * intros [|f]; [done |].
+    unfold union, perm_union; simpl. f_equal. apply perm_union_half.
+Qed.
