empty_permissions.v
@@ -5,42 +5,23 @@ system with no permissions at all. The permission kind is [Free] (i.e.
 everything is allowed), and all operations are no-ops.*)
 Require Export abstract_permissions.
 
-Instance unit_perm_kind: PermKind unit := λ _, Free.
-Instance unit_perm_lock: PermLock unit := λ _ _, ().
-
-Inductive unit_subseteq: SubsetEq unit :=
-  | tt_subseteq : () ⊆ ().
-Existing Instance unit_subseteq.
-
-Inductive unit_disjoint: Disjoint unit := .
-Existing Instance unit_disjoint.
-
-Instance unit_union: Union unit := λ _ _, ().
-Instance unit_difference: Difference unit := λ _ _, ().
-
-Instance unit_subseteq_dec (u1 u2 : unit) : Decision (u1 ⊆ u2).
-Proof. left. by destruct u1, u2. Defined.
-Instance unit_disjoint_dec (u1 u2 : unit) : Decision (u1 ⊥ u2).
-Proof. right. destruct 1. Defined.
+Instance unit_perm_ops: PermissionsOps unit := {
+  perm_kind := λ _, Free;
+  perm_lock_ := λ _ _, ();
+  perm_subseteq := λ _ _, True;
+  perm_disjoint := λ _ _, False;
+  perm_union := λ _ _, ();
+  perm_difference := λ _ _, ()
+}.
 
 Instance: Permissions unit.
 Proof.
-  split.
+  split; try done.
   * repeat split; by repeat intros [].
-  * destruct 1.
-  * by destruct 1.
-  * intros ? [? []].
-  * destruct 1.
-  * by intros [].
-  * by intros [].
-  * by intros [].
-  * by intros [] [] [].
   * by intros [] [].
-  * destruct 1.
-  * destruct 1.
-  * destruct 1.
-  * by intros [] [] [].
-  * destruct 1.
+  * by intros [] [??].
+  * by intros [].
+  * by intros [].
   * by intros [] [] [? []].
   * by intros [] [] [? []].
 Qed.
